Std/Classes/BEq.lean
@@ -1,0 +1,23 @@
+/-
+Copyright (c) 2022 Mario Carneiro. All rights reserved.
+Released under Apache 2.0 license as described in the file LICENSE.
+Authors: Mario Carneiro
+-/
+
+/-! ## Boolean equality -/
+
+/-- `PartialEquivBEq α` says that the `BEq` implementation is a
+partial equivalence relation, that is:
+* it is symmetric: `a == b → b == a`
+* it is transitive: `a == b → b == c → a == c`.
+-/
+class PartialEquivBEq (α) [BEq α] : Prop where
+  /-- Symmetry for `BEq`. If `a == b` then `b == a`. -/
+  symm : (a : α) == b → b == a
+  /-- Transitivity for `BEq`. If `a == b` and `b == c` then `a == c`. -/
+  trans : (a : α) == b → b == c → a == c
+
+@[simp] theorem beq_eq_false_iff_ne [BEq α] [LawfulBEq α]
+    (a b : α) : (a == b) = false ↔ a ≠ b := by
+  rw [ne_eq, ← beq_iff_eq a b]
+  cases a == b <;> decide
