Std/Data/Array/Lemmas.lean
@@ -53,6 +53,9 @@ theorem get?_len_le (a : Array α) (i : Nat) (h : a.size ≤ i) : a[i]? = none :
 theorem getElem_eq_data_get (a : Array α) (h : i < a.size) : a[i] = a.data.get ⟨i, h⟩ := by
   by_cases i < a.size <;> simp [*] <;> rfl
 
+theorem getElem_mem_data (a : Array α) (h : i < a.size) : a[i] ∈ a.data := by
+  simp [getElem_eq_data_get, List.get_mem]
+
 theorem getElem?_eq_data_get? (a : Array α) (i : Nat) : a[i]? = a.data.get? i := by
   by_cases i < a.size <;> simp_all [getElem?_pos, getElem?_neg, List.get?_eq_get, eq_comm] <;> rfl
 
