Std/Data/List/Lemmas.lean
@@ -6,6 +6,7 @@ Authors: Parikshit Khanna, Jeremy Avigad, Leonardo de Moura, Floris van Doorn, M
 import Std.Data.Nat.Lemmas
 import Std.Data.List.Basic
 import Std.Data.Option.Lemmas
+import Std.Classes.BEq
 
 namespace List
 
@@ -770,6 +771,10 @@ theorem set_comm (a b : α) : ∀ {n m : Nat} (l : List α), n ≠ m →
     (hj : j < (l.set i a).length) :
     (l.set i a).get ⟨j, hj⟩ = l.get ⟨j, by simp at hj; exact hj⟩ := by
   rw [← Option.some_inj, ← List.get?_eq_get, List.get?_set_ne _ _ h, List.get?_eq_get]
+
+theorem get_set (a : α) {m n} (l : List α) (h) :
+    (set l m a).get ⟨n, h⟩ = if m = n then a else l.get ⟨n, length_set .. ▸ h⟩ := by
+  if h : m = n then subst m; simp else simp [h]
 
 theorem mem_or_eq_of_mem_set : ∀ {l : List α} {n : Nat} {a b : α}, a ∈ l.set n b → a ∈ l ∨ a = b
   | _ :: _, 0, _, _, h => ((mem_cons ..).1 h).symm.imp_left (.tail _)
